Lax KS

src/tls/KeySchedule.fst
@@ -138,14 +138,13 @@ private let res_psk_value (i:rmsId{registered_res_psk i}) =
 abstract let psk (i:esId) =
   b:bytes{length b = hashSize (esId_hash i)}
 
-let get_psk_info (i:esId) =
+let read_psk (i:esId) : ST (psk i * Hashing.Spec.alg * aeadAlg)
+  (requires fun h -> True)
+  (ensures fun h0 _ h1 -> modifies_none h0 h1) =
   match i with
-  | ApplicationPSK i _ -> PSK.psk_info i
-
-private let get_psk (i:esId) =
-  match i with
-  | ApplicationPSK pskid _ ->
-     let p : psk i = psk_value pskid in p
+  | ApplicationPSK i h ->
+    let c = PSK.psk_info i in
+    (PSK.psk_value i, c.early_hash, c.early_ae)
 
 // Agile "0" hash
 private let zH h : St (Hashing.Spec.tag h) =
@@ -357,7 +356,7 @@ let ks_client_13_1rtt_init ks gl =
     let (| g, gx |) = gx in
     match CommonDH.namedGroup_of_group g with
     | None -> None // Impossible
-    | Some ng -> Some (ng, CommonDH.serialize_raw #g gx) in
+    | Some ng -> Some (CommonDH.Share g gx) in
   let serialized = List.Tot.choose serialize_share gs in
   CommonDH.ClientKeyShare serialized
 
@@ -386,14 +385,13 @@ let ks_client_13_0rtt_init ks esId gl =
     let (| g, gx |) = gx in
     match CommonDH.namedGroup_of_group g with
     | None -> None // Impossible
-    | Some ng -> Some (ng, CommonDH.serialize_raw #g gx) in
+    | Some ng -> Some (CommonDH.Share g gx) in
   let serialized = List.Tot.choose serialize_share gs in
   CommonDH.ClientKeyShare serialized
 
 
 // Derive the early keys from the early secret
-let ks_client_13_0rtt_ch ks esId
-  : ST (recordInstance * recordInstance)
+let ks_client_13_0rtt_ch ks esId : ST (recordInstance)
   (requires fun h0 ->
     let kss = sel h0 (KS?.state ks) in
     C? kss /\ C_Init? (C?.s kss))
@@ -403,14 +401,12 @@ let ks_client_13_0rtt_ch ks esId
     /\ modifies_rref rid !{as_ref st} (HS.HS?.h h0) (HS.HS?.h h1)) =
   let KS #rid st hsl = ks in
   let C (C_13_wait_CH cr esId gs) = !st in
-  let psk = get_psk esId in
-  let c = get_psk_info esId in
-  let h, ae = c.early_hash, c.early_ae in
+  let psk, h, ae = read_psk esId in
 
-  let expandId = EarlySecretID esId in
-  let loginfo = LogInfo_CH ({li_ch_cr = cr; li_ch_psk = c}) in
+  let secretId = EarlySecretID esId in
+  let loginfo = LogInfo_CH ({li_ch_cr = cr; li_ch_psk=[]}) in
   let hashed_log = HandshakeLog.getHash hsl h in
-  // TODO verify log_info loginfo hashed_log
+  let expandId = ExpandedSecret secretId EarlyTrafficSecret loginfo hashed_log in
 
   let hL = hashSize h in
   let zeroes = Platform.Bytes.abytes (String.make hL (Char.char_of_int 0)) in
@@ -426,13 +422,6 @@ let ks_client_13_0rtt_ch ks esId
   let (cfk0, _) = finished_13 h es_derived in
   let cfk0 : fink efId = cfk0 in
 
-  let id = ID13 (KeyID expandId EarlyTrafficKey Client loginfo hashed_log) in
-  let ckv: StreamAE.key id = ck in
-  let civ: StreamAE.iv id  = civ in
-  let rw = StAE.coerce HyperHeap.root id (ckv @| civ) in
-  let r = StAE.genReader HyperHeap.root rw in
-  let early_hs = StAEInstance r rw in
-
   let id = ID13 (KeyID expandId EarlyApplicationDataKey Client loginfo hashed_log) in
   let ckv: StreamAE.key id = ck' in
   let civ: StreamAE.iv id  = civ' in
@@ -441,7 +430,7 @@ let ks_client_13_0rtt_ch ks esId
   let early_d = StAEInstance r rw in
 
   st := C (C_13_wait_SH cr (Some (| esId, es |)) (Some (| efId, cfk0 |)) gs);
-  (early_hs, early_d)
+  (early_d)
 
 val ks_client_13_0rtt_finished: ks:ks -> ST (cvd:bytes)
   (requires fun h0 ->
@@ -504,7 +493,7 @@ let ks_server_12_init_dh ks cr pv cs ems g =
   st := S (S_12_wait_CKE_DH csr (pv, cs, ems) (| g, our_share |));
   CommonDH.pubshare our_share
 
-val ks_server_13_0rtt_init: ks:ks -> cr:random -> i:esId -> cs:cipherSuite -> g:CommonDH.group -> gx:CommonDH.share g -> ST (recordInstance * recordInstance * our_share:CommonDH.share g)
+val ks_server_13_0rtt_init: ks:ks -> cr:random -> i:esId -> cs:cipherSuite -> g:CommonDH.group -> gx:CommonDH.share g -> ST (recordInstance * our_share:CommonDH.share g)
   (requires fun h0 ->
     let kss = sel h0 (KS?.state ks) in
     S? kss /\ S_Init? (S?.s kss)
@@ -518,19 +507,16 @@ val ks_server_13_0rtt_init: ks:ks -> cr:random -> i:esId -> cs:cipherSuite -> g:
 let ks_server_13_0rtt_init ks cr esId cs g gx =
   let KS #region st hsl = ks in
   let S (S_Init sr) = !st in
-  let psk = get_psk esId in
-  let c = get_psk_info esId in
-  let h: TLSConstants.hash_alg = c.early_hash in
-  let ae = c.early_ae in
+  let psk, h, ae = read_psk esId in
 
   let hL = hashSize h in
   let zeroes = Platform.Bytes.abytes (String.make hL (Char.char_of_int 0)) in
   let es : es esId = HKDF.hkdf_extract h zeroes psk in
 
-  let expandId = EarlySecretID esId in
-  let loginfo = LogInfo_CH ({li_ch_cr = cr; li_ch_psk = c}) in
+  let secretId = EarlySecretID esId in
+  let loginfo = LogInfo_CH ({li_ch_cr = cr; li_ch_psk=[]}) in
   let hashed_log = HandshakeLog.getHash hsl h in
-  // TODO verify log_info loginfo hashed_log
+  let expandId = ExpandedSecret secretId EarlyTrafficSecret loginfo hashed_log in
 
   let sh_rctx = hashed_log @| (esId_rc esId) in
   let es_derived = HKDF.hkdf_expand_label h es "early traffic secret" sh_rctx hL in
@@ -541,13 +527,6 @@ let ks_server_13_0rtt_init ks cr esId cs g gx =
   let (cfk0, _) = finished_13 h es_derived in
   let cfk0 : fink efId = cfk0 in
 
-  let id = ID13 (KeyID expandId EarlyTrafficKey Client loginfo hashed_log) in
-  let ckv: StreamAE.key id = ck in
-  let civ: StreamAE.iv id  = civ in
-  let rw = StAE.coerce HyperHeap.root id (ckv @| civ) in
-  let r = StAE.genReader HyperHeap.root rw in
-  let early_hs = StAEInstance r rw in
-
   let id = ID13 (KeyID expandId EarlyApplicationDataKey Client loginfo hashed_log) in
   let ckv: StreamAE.key id = ck' in
   let civ: StreamAE.iv id  = civ' in
@@ -556,10 +535,10 @@ let ks_server_13_0rtt_init ks cr esId cs g gx =
   let early_d = StAEInstance r rw in
 
   let gy, gxy = CommonDH.dh_responder gx in
-  let hsId = HSID_PSK_DHE esId g gx gy in
+  let hsId = HSID_DHE (EarlySalt esId) g gx gy in
   let hs : hs hsId = HKDF.hkdf_extract h es gxy in
   st := S (S_13_wait_SH (ae, h) cr sr (Some (| esId, es |)) (Some (| efId, cfk0 |)) (| hsId, hs |));
-  early_hs, early_d, gy
+  early_d, gy
 
 val ks_server_13_1rtt_psk_init: ks:ks -> cr:random -> cs:cipherSuite -> ST unit
   (requires fun h0 ->
@@ -593,15 +572,15 @@ let ks_server_13_1rtt_init ks cr cs g gx =
   let S (S_Init sr) = !st in
   let CipherSuite _ _ (AEAD ae h) = cs in
   let gy, gxy = CommonDH.dh_responder gx in
-  let hsId = HSID_DHE h g gx gy in
+  let esId = NoPSK h in
+  let hsId = HSID_DHE (EarlySalt esId) g gx gy in
   let hL = hashSize h in
   let zeroes = Platform.Bytes.abytes (String.make hL (Char.char_of_int 0)) in
   let es = HKDF.hkdf_extract h zeroes zeroes in
   let hs : hs hsId = HKDF.hkdf_extract h es gxy in
   st := S (S_13_wait_SH (ae, h) cr sr None None (| hsId, hs |));
-
   match CommonDH.namedGroup_of_group g with
-  | Some gn -> CommonDH.ServerKeyShare (gn, CommonDH.serialize_raw #g gy)
+  | Some gn -> CommonDH.ServerKeyShare (CommonDH.Share g gy)
 
 val ks_server_13_sh: ks:ks -> ST recordInstance
   (requires fun h0 ->
@@ -615,14 +594,16 @@ val ks_server_13_sh: ks:ks -> ST recordInstance
 let ks_server_13_sh ks =
   let KS #region st hsl = ks in
   let S (S_13_wait_SH (ae, h) cr sr _ _ (| hsId, hs |)) = !st in
-  let expandId = HandshakeSecretID hsId in
+  let secretId = HandshakeSecretID hsId in
   let loginfo = LogInfo_SH ({
     li_sh_cr = cr;
     li_sh_sr = sr;
     li_sh_ae = AEAD ae h;
+    li_sh_hash = h;
+    li_sh_psk = None;
   }) in
   let hashed_log = HandshakeLog.getHash hsl h in
-  // TODO log_info loginfo hashed_log
+  let expandId = ExpandedSecret secretId HandshakeTrafficSecret loginfo hashed_log in
 
   // Derived handshake secret
   let hL = hashSize h in
@@ -649,7 +630,7 @@ let ks_server_13_sh ks =
   let sfk1 : fink sfkId = sfk1 in
 
   // Replace handshake secret with application master secret
-  let amsId = ASID hsId in
+  let amsId = ASID (HandshakeSalt hsId) in
   let ams : ams amsId = HKDF.hkdf_extract h hs zeroes in
 
   st := S (S_13_wait_SF (ae, h) (| cfkId, cfk1 |) (| sfkId, sfk1 |) (| amsId, ams |));
@@ -722,7 +703,7 @@ let ks_client_12_resume ks sr pv cs =
 //   2. they use different return types
 //   3. they are called at different locations
 
-val ks_client_13_sh: ks:ks -> cs:cipherSuite -> g:CommonDH.group -> gy:CommonDH.share g -> accept_early_data:bool -> ST recordInstance
+val ks_client_13_sh: ks:ks -> sr:random -> cs:cipherSuite -> g:CommonDH.group -> gy:CommonDH.share g -> accept_early_data:bool -> ST recordInstance
   (requires fun h0 ->
     let kss = sel h0 (KS?.state ks) in
     C? kss /\ C_13_wait_SH? (C?.s kss) /\
@@ -741,7 +722,7 @@ val ks_client_13_sh: ks:ks -> cs:cipherSuite -> g:CommonDH.group -> gy:CommonDH.
     /\ modifies_rref rid !{as_ref st} (HS.HS?.h h0) (HS.HS?.h h1))
 
 // ServerHello log breakpoint (client)
-let ks_client_13_sh ks cs g gy accept_ed =
+let ks_client_13_sh ks sr cs g gy accept_ed =
   let KS #region st hsl = ks in
   let C (C_13_wait_SH cr early_info early_fin gc) = !st in
   let Some gx = List.Tot.find (fun (gx:(x:CommonDH.group & CommonDH.share g)) -> let (| g', _ |) = gx in g = g') gc in
@@ -749,24 +730,28 @@ let ks_client_13_sh ks cs g gy accept_ed =
   let gxy = CommonDH.dh_initiator #g gx gy in
   let CipherSuite _ _ (AEAD ae h) = cs in
   let gx = CommonDH.pubshare gx in // Forget the private exponent
-
-  let loginfo = LogInfo_SH ({li_sh_cr = cr; li_sh_sr = cr; li_sh_ae = AEAD ae h;}) in // TODO
-  let hashed_log = HandshakeLog.getHash hsl h in
   let hL = hashSize h in
   let zeroes = Platform.Bytes.abytes (String.make hL (Char.char_of_int 0)) in
 
   // Early secret: must derive zero here as hash is not known before
-  let es =
+  let esId, es =
     match early_info, accept_ed with
-    | Some (| _, es |), true -> es
-    | _ -> HKDF.hkdf_extract h zeroes zeroes
+    | Some (| i, es |), true -> i, es
+    | _ -> NoPSK h, HKDF.hkdf_extract h zeroes zeroes
   in
 
-  let hsId = match early_info with
-    | None -> HSID_DHE h g gx gy
-    | Some (| esId, _ |) -> HSID_PSK_DHE esId g gx gy in
+  let hsId = HSID_DHE (EarlySalt esId) g gx gy in
   let hs : hs hsId = HKDF.hkdf_extract h es gxy in
-  let expandId = HandshakeSecretID hsId in
+  let secretId = HandshakeSecretID hsId in
+  let loginfo = LogInfo_SH ({
+    li_sh_cr = cr;
+    li_sh_sr = sr;
+    li_sh_ae = AEAD ae h;
+    li_sh_hash = h;
+    li_sh_psk = None;
+  }) in
+  let hashed_log = HandshakeLog.getHash hsl h in
+  let expandId = ExpandedSecret secretId HandshakeTrafficSecret loginfo hashed_log in
 
   // Derived handshake secret
   let sh_rctx = hashed_log @| (hsId_rc hsId) in
@@ -781,7 +766,7 @@ let ks_client_13_sh ks cs g gy accept_ed =
   let sfk1 : fink sfkId = sfk in
 
   // Application master secret
-  let asId = ASID hsId in
+  let asId = ASID (HandshakeSalt hsId) in
   let ams : ams asId = HKDF.hkdf_extract h hs zeroes in
 
   let id = ID13 (KeyID expandId HandshakeKey Client loginfo hashed_log) in
@@ -865,10 +850,11 @@ let ks_client_13_sf ks
   let (ae, h) = alpha in
   let (| FinishedID _ _ _ loginfo _, _ |) = cfk in // TODO loginfo
 
-  let expandId = ApplicationSecretID asId in
+  let secretId = ApplicationSecretID asId in
   let hashed_log = HandshakeLog.getHash hsl h in
   let hL = hashSize h in
   let zeroes = Platform.Bytes.abytes (String.make hL (Char.char_of_int 0)) in
+  let expandId = ExpandedSecret secretId ApplicationTrafficSecret loginfo hashed_log in
 
   // Derived applcation master secret
   let sh_rctx = hashed_log @| (asId_rc asId) in
@@ -881,7 +867,7 @@ let ks_client_13_sf ks
   let late_cfk: fink cfkId = late_cfk in
 
   // Rekeying secret
-  let ri = RekeyID asId loginfo hashed_log 1 in
+  let ri = expandId in
   let rk1 : rekey_secret ri = HKDF.hkdf_expand_label h ams_derived "application traffic secret" empty_bytes hL in
 
   let id = ID13 (KeyID expandId ApplicationDataKey Client loginfo hashed_log) in
@@ -911,10 +897,11 @@ let ks_server_13_sf ks
   let (| FinishedID _ _ _ loginfo _, _ |) = cfk in // TODO loginfo
   let (ae, h) = alpha in
 
-  let expandId = ApplicationSecretID asId in
+  let secretId = ApplicationSecretID asId in
   let hashed_log = HandshakeLog.getHash hsl h in
   let hL = hashSize h in
   let zeroes = Platform.Bytes.abytes (String.make hL (Char.char_of_int 0)) in
+  let expandId = ExpandedSecret secretId ApplicationTrafficSecret loginfo hashed_log in
 
   // Derived applcation master secret
   let sh_rctx = hashed_log @| (asId_rc asId) in
@@ -927,7 +914,7 @@ let ks_server_13_sf ks
   let late_cfk: fink cfkId = late_cfk in
 
   // Rekeying secret
-  let ri = RekeyID asId loginfo hashed_log 1 in
+  let ri = expandId in //RekeyID asId loginfo hashed_log 1 in
   let rk1 : rekey_secret ri = HKDF.hkdf_expand_label h ams_derived "application traffic secret" empty_bytes hL in
 
   let id = ID13 (KeyID expandId ApplicationDataKey Server loginfo hashed_log) in
